Arreglado lo de mayor que cero en vez de uno

ocaml_interface/checker.ml
@@ -1035,7 +1035,7 @@ module Parser =
  
 let filename = "example.txt"    
 
-let read_lines name : char list list =
+let read_lines name : string list =
   let ic = open_in name in
   let try_read () =
     try Some (input_line ic) with End_of_file -> None in
@@ -1044,6 +1044,12 @@ let read_lines name : char list list =
     | None -> close_in ic; List.rev acc in
   loop []
   
+let explode s : char list =
+  let rec exp i l =
+    if i < 0 then l else exp (i - 1) (s.[i] :: l) in
+  exp (String.length s - 1) []
+
+  
 let rec print_list = function 
 [] -> ()
 | e::l -> print_string e ; print_string "\n" ; print_list l
@@ -1051,8 +1057,8 @@ let rec print_list = function
 let () = 
 try
     let lines = read_lines filename in
-    let res = check_loop (List.map tokenize lines) in
-    printf("Resultado: ");
-    printf(res);
+    let res = Parser.check_loop (List.map Parser.tokenize (List.map explode lines))   in
+    print_string("Resultado: ");
+    if res then print_string("Todo correcto\n") else print_string("Ha ocurrido un error\n");
     flush stdout
 with e -> raise e
