ocaml_interface/main.ml
@@ -1,4 +1,4 @@
-
+ 
 let filename = "example.txt"    
 
 let read_lines name : string list =
@@ -10,6 +10,12 @@ let read_lines name : string list =
     | None -> close_in ic; List.rev acc in
   loop []
   
+let explode s : char list =
+  let rec exp i l =
+    if i < 0 then l else exp (i - 1) (s.[i] :: l) in
+  exp (String.length s - 1) []
+
+  
 let rec print_list = function 
 [] -> ()
 | e::l -> print_string e ; print_string "\n" ; print_list l
@@ -17,7 +23,8 @@ let rec print_list = function
 let () = 
 try
     let lines = read_lines filename in
-    print_list lines;
-    flush stdout;
-    let res = check_loop
+    let res = Parser.check_loop (List.map Parser.tokenize (List.map explode lines))   in
+    print_string("Resultado: ");
+    if res then print_string("Todo correcto") else print_string("Ha ocurrido un error");
+    flush stdout
 with e -> raise e
